src/goose_lang/dist_lifting.v
@@ -17,14 +17,20 @@ Context `{@ffi_interp_adequacy ffi interp ext ffi_sem}.
 Class heap_globalG Σ := {
   heap_globalG_preG :> heapPreG Σ;
   heap_globalG_names : ffi_global_names;
+  heap_globalG_inv_names : inv_names;
+  (*
   heap_globalG_invG :> invG Σ;
+   *)
 }.
+
+Global Instance heap_globalG_invG {Σ} {hgG: heap_globalG Σ} : invG Σ :=
+  inv_update_pre (heap_preG_iris) (heap_globalG_inv_names).
 
 Program Global Instance heapG_groveG `{!heap_globalG Σ} : groveG goose_lang goose_crash_lang Σ :=
 {
   grove_global_state_interp := λ g κs n, ffi_pre_global_ctx Σ (heap_preG_ffi) (heap_globalG_names) g;
   grove_num_laters_per_step := λ n, 1%nat;
-  grove_invG := heap_globalG_invG;
+  grove_invG := heap_globalG_invG
 }.
 
 Definition hgG_extend_local_names {Σ} (hgG : heap_globalG Σ) (names : heap_local_names) : heap_names :=
@@ -34,7 +40,9 @@ Definition hgG_extend_local_names {Σ} (hgG : heap_globalG Σ) (names : heap_loc
      heap_ffi_global_names := heap_globalG_names |}.
 
 Definition heap_globalG_heapG {Σ} (hgG: heap_globalG Σ) (Hc: crashG Σ) (names: heap_local_names) : heapG Σ :=
-  heap_update_pre Σ (heap_globalG_preG) (heap_globalG_invG) Hc (hgG_extend_local_names hgG names).
+  heap_update_pre Σ (heap_globalG_preG) (heap_globalG_invG)
+                  {| crash_inG := (@crash_inPreG _ heap_preG_crash); crash_name := @crash_name _ Hc |}
+                  (hgG_extend_local_names hgG names).
 
 Definition wpd `{hgG: !heap_globalG Σ} (k: nat) (E: coPset)
            (cts: list (crashG Σ * heap_local_names)) (ers: list (expr * expr)) :=
