src/goose_lang/dist_adequacy.v
@@ -12,7 +12,8 @@ Set Default Proof Using "Type".
 Theorem heap_dist_adequacy `{ffi_sem: ffi_semantics} `{!ffi_interp ffi} {Hffi_adequacy:ffi_interp_adequacy}
         Σ `{hPre: !heapPreG Σ} k (ebσs : list node_init_cfg)
         g φinv (HINITG: ffi_initgP g) (HINIT: ∀ σ, σ ∈ init_local_state <$> ebσs → ffi_initP σ.(world) g) :
-  (∀ `{Hheap : !heap_globalG Σ} (cts : list (crashG Σ * heap_local_names)),
+  (∀ `{Hheap : !heap_globalG Σ} (cts : list (crashG Σ * heap_local_names))
+      (Heq_cts: ∀ k ct, cts !! k = Some ct → @crash_inG _ (fst ct) = crash_inPreG),
       ⊢
         ffi_pre_global_start Σ (heap_preG_ffi (heapPreG := heap_globalG_preG)) (heap_globalG_names) g ={⊤}=∗
         ([∗ list] i ↦ ct; σ ∈ cts; init_local_state <$> ebσs,
@@ -24,11 +25,12 @@ Theorem heap_dist_adequacy `{ffi_sem: ffi_semantics} `{!ffi_interp ffi} {Hffi_ad
 Proof.
   intros Hwp.
   eapply (wpd_dist_adequacy_inv _ _ _ heap_local_namesO).
-  iIntros (Hinv ?) "".
+  iIntros (Hinv Heq_inv ?) "".
   iMod (ffi_name_global_init _ _ g) as (ffi_namesg) "(Hgw&Hgstart)"; first auto.
   set (hgG := {| heap_globalG_preG := _; heap_globalG_names := ffi_namesg;
-                     heap_globalG_invG := Hinv |}).
-  iAssert (|==> ∃ cts, ffi_pre_global_ctx Σ heap_preG_ffi ffi_namesg g ∗
+                     heap_globalG_inv_names := inv_get_names Hinv |}).
+  iAssert (|==> ∃ cts (Heq_cts: ∀ k ct, cts !! k = Some ct → @crash_inG _ (fst ct) = crash_inPreG),
+              ffi_pre_global_ctx Σ heap_preG_ffi ffi_namesg g ∗
               ([∗ list] i ↦ ct; σ ∈ cts; init_local_state <$> ebσs,
               let hG := heap_globalG_heapG hgG (fst ct) (snd ct) in
               NC 1 ∗ state_interp σ 0) ∗
@@ -40,34 +42,49 @@ Proof.
   { clear -HINIT. remember (init_local_state <$> ebσs) as σs eqn:Heq. clear Heq.
     iInduction σs as [| σ σs] "IH".
     { iExists []; eauto. }
-    { iMod ("IH" with "[] [$]") as (cts) "(Hpre&H1&H2)".
+    { iMod ("IH" with "[] [$]") as (cts Heq_cts) "(Hpre&H1&H2)".
       { iPureIntro. intros. eapply HINIT. set_solver. }
       iMod (na_heap_name_init tls σ.(heap)) as (name_na_heap) "Hh".
       iMod (ffi_name_init _ _ σ.(world) g with "[$]") as (ffi_names) "(Hw&Hgw&Hstart)"; first auto.
       { eapply HINIT. set_solver. }
       iMod (trace_name_init σ.(trace) σ.(oracle)) as (name_trace) "(Htr&Htrfrag&Hor&Hofrag)".
-      iMod (NC_alloc) as (Hc) "HNC".
+      iMod (NC_alloc_strong) as (γn) "HNC".
       set (hnames := {| heap_local_heap_names := name_na_heap;
                       heap_local_ffi_local_names := ffi_names;
                       heap_local_trace_names := name_trace |}).
-      iExists ((Hc, hnames) :: cts).
+      iExists (({| crash_name := γn |}, hnames) :: cts).
       iModIntro. iFrame.
       rewrite ffi_pre_global_ctx_spec /=. eauto.
     }
   }
-  iMod "H" as (cts) "(Hgw&Hres1&Hres2)".
+  iMod "H" as (cts Heq_cts) "(Hgw&Hres1&Hres2)".
   iExists ((λ x, (fst x, {| pbundleT := snd x |})) <$> cts).
   (* XXX: we need an Hc floating about below because heap_update_pre expects one, but it is
           not really needed. *)
-  iMod (NC_alloc) as (Hc) "_".
+  iMod (NC_alloc_strong) as (γn) "_".
+  unshelve (iExists _).
+  { intros k' ct Hlookup.
+    rewrite list_lookup_fmap in Hlookup.
+    apply fmap_Some_1 in Hlookup as ((Hc&t)&Hlookup1&Heq1).
+    specialize (Heq_cts k' (Hc, t)). rewrite Heq1. rewrite Heq_cts; eauto. }
   iExists
-    (λ t σ nt, let _ := heap_globalG_heapG hgG Hc (@pbundleT _ _ t) in
+    (λ t σ nt, let _ := heap_globalG_heapG hgG {| crash_name := γn |} (@pbundleT _ _ t) in
                state_interp σ nt)%I.
   iExists
     (λ g ns κs, ffi_pre_global_ctx Σ heap_preG_ffi ffi_namesg g).
   iExists (λ _ _, True)%I.
   unshelve (iExists _, _, _, _); eauto.
-  iMod (Hwp hgG with "[$] [$]") as ">(H1&Hwp)".
+  iPoseProof (Hwp hgG with "[$] [$]") as "Hwp".
+  { eauto. }
+  assert ((@grove_invG (@goose_lang ext ffi ffi_sem) (@goose_crash_lang ext ffi ffi_sem) Σ
+                      (@heapG_groveG ext ffi ffi_sem ffi_interp0 Hffi_adequacy Σ hgG)) =
+          Hinv) as ->.
+  { rewrite /grove_invG/heapG_groveG.
+    rewrite /heap_globalG_invG.
+    rewrite /inv_update_pre.
+    destruct Hinv. f_equal.
+    eauto. }
+  iMod "Hwp" as ">(H1&Hwp)".
   iModIntro.
   iSplitL "H1".
   {  iIntros (???) "Hσ".
@@ -76,7 +93,13 @@ Proof.
   }
   iFrame "Hgw".
   iSplitL "Hres1".
-  { rewrite ?big_sepL2_fmap_r ?big_sepL2_fmap_l. eauto. }
+  { rewrite ?big_sepL2_fmap_r ?big_sepL2_fmap_l. eauto.
+    iApply (big_sepL2_mono with "Hres1").
+    iIntros (??? Hlookup1 Hlookup2) "(HNC&$)".
+    eapply Heq_cts in Hlookup1.
+    iExactEq "HNC". f_equal. rewrite //=.
+    destruct y1; eauto => //=.
+    rewrite //= in Hlookup1. destruct c. rewrite -Hlookup1 //=. }
   rewrite /wpd/dist_weakestpre.wpd.
   iSplit.
   { iModIntro. iIntros (ct Hin). iSplit; first eauto.
@@ -85,7 +108,7 @@ Proof.
   iApply (big_sepL2_mono with "Hwp").
   iIntros (k' (Hc'&Hnames) ρ Hin1 Hin2) "H".
   iDestruct "H" as (Φ Φrx Φinv) "Hwpr".
-  set (hG := heap_globalG_heapG hgG Hc Hnames).
+  set (hG := heap_globalG_heapG hgG {| crash_name := γn |} Hnames).
   iExists Φ, (λ Hc names v, Φrx (heap_update_local _ hG _ Hc (@pbundleT _ _ names)) v),
     (λ Hc names, Φinv (heap_update_local _ hG _ Hc (@pbundleT _ _ names))).
   rewrite /wpr//=.
@@ -96,15 +119,59 @@ Proof.
     rewrite ffi_update_pre_get_local; eauto. destruct heap_local_heap_names; eauto. }
   rewrite Heqnames.
   iDestruct (wpr_proper_irisG_equiv with "Hwpr") as "Hwpr"; last first.
-  { iApply (@recovery_weakestpre.wpr_strong_mono with "Hwpr []").
+  {
+    assert (Hc' = {| crash_inG := crash_inPreG; crash_name := crash_name |}) as <-.
+    {
+      eapply Heq_cts in Hin1.
+      destruct Hc'; eauto => //=.
+      rewrite //= in Hin1. rewrite -Hin1 //=. }
+    iApply (@recovery_weakestpre.wpr_strong_mono with "Hwpr []").
     iSplit; eauto.
-    iModIntro. iSplit; eauto. }
-  clear.
+    iModIntro.
+    assert (Hc' = {| crash_inG := crash_inPreG; crash_name := crash_name |}) as Heq_c'.
+    {
+      eapply Heq_cts in Hin1.
+      destruct Hc'; eauto => //=.
+      rewrite //= in Hin1. rewrite -Hin1 //=. }
+    iSplit; eauto.
+    { iIntros (??) "H". iExactEq "H". f_equal. rewrite /hG.
+      rewrite Heq_c'.
+      rewrite /heap_update_local. f_equal.
+      { rewrite /heapG_irisG//=.
+        transitivity (@heap_globalG_invG ext ffi ffi_sem ffi_interp0 Hffi_adequacy Σ hgG); first done.
+        rewrite /heap_globalG_invG.
+        rewrite /inv_update_pre.
+        destruct Hinv. f_equal.
+        eauto. }
+    }
+    { iIntros (???) "H". iModIntro. iExactEq "H". f_equal. rewrite /hG.
+      rewrite Heq_c'.
+      rewrite /heap_update_local. f_equal.
+      { rewrite /heapG_irisG//=.
+        transitivity (@heap_globalG_invG ext ffi ffi_sem ffi_interp0 Hffi_adequacy Σ hgG); first done.
+        rewrite /heap_globalG_invG.
+        rewrite /inv_update_pre.
+        destruct Hinv. f_equal.
+        eauto. }
+    }
+  }
+  clear -Heq_inv.
   intros Hcnew tnew.
   split_and!; eauto.
+  - transitivity ( @heap_globalG_invG ext ffi ffi_sem ffi_interp0 Hffi_adequacy Σ hgG); first done.
+    transitivity (Hinv); last done.
+    rewrite /heap_globalG_invG.
+    rewrite /inv_update_pre.
+    destruct Hinv. f_equal.
+    eauto.
   - rewrite //= ffi_update_pre_update. eauto.
   - rewrite //= ffi_update_pre_update.
     iIntros. rewrite ffi_pre_global_ctx_spec; eauto.
+    Unshelve.
+    { intros ?? Hfalse. rewrite lookup_nil in Hfalse. congruence. }
+    { intros ?? Hlookup. destruct k.
+      - rewrite /= in Hlookup. inversion Hlookup; subst => //=.
+      - rewrite /= in Hlookup. eauto. }
 Qed.
 
 (* This version might be more useful. Rather than assembling a wpd explicitly
@@ -121,7 +188,7 @@ Theorem heap_dist_adequacy_alt `{ffi_sem: ffi_semantics} `{!ffi_interp ffi} {Hff
               let e := init_thread ebσ in
               let r := init_restart ebσ in
               let σ := init_local_state ebσ in
-              ∀ Hcrash local_names,
+              ∀ Hcrash (Heq: @crash_inG _ Hcrash = crash_inPreG) local_names,
               let hG := heap_globalG_heapG Hheap Hcrash local_names in
               ffi_local_start (heapG_ffiG) σ.(world) g ∗
               trace_frag σ.(trace) ∗ oracle_frag σ.(oracle) ={⊤}=∗
@@ -131,7 +198,7 @@ Theorem heap_dist_adequacy_alt `{ffi_sem: ffi_semantics} `{!ffi_interp ffi} {Hff
 Proof.
   intros Hwp.
   eapply (heap_dist_adequacy _ k); eauto.
-  iIntros (??) "H".
+  iIntros (???) "H".
   iMod (Hwp with "[$]") as "(Hwprs&Hinv)".
   iModIntro. iIntros "H". iFrame "Hinv".
   rewrite /wpd.
@@ -144,9 +211,11 @@ Proof.
   iApply (big_sepL_mono with "H").
   iIntros (i ρ Hlookup) "(Hwand&Hres)".
   iDestruct "Hres" as (ct Hlookup2) "Hres".
-  iMod ("Hwand" $! (fst ct) (snd ct) with "[$]") as "H".
+  iMod ("Hwand" $! (fst ct) _ (snd ct) with "[$]") as "H".
   iModIntro. iExists _; iSplit; eauto.
   rewrite //=. iDestruct "H" as (???) "H". iExists _, _, _. iFrame.
+  Unshelve.
+  { eapply Heq_cts in Hlookup2. eauto. }
 Qed.
 
 Section failstop.
@@ -172,7 +241,7 @@ Theorem heap_dist_adequacy_failstop
         ([∗ list] ebσ ∈ ebσs,
               let e := fst ebσ in
               let σ := snd ebσ in
-              ∀ Hcrash local_names,
+              ∀ Hcrash (Heq: @crash_inG _ Hcrash = crash_inPreG) local_names,
               let hG := heap_globalG_heapG Hheap Hcrash local_names in
               ffi_local_start (heapG_ffiG) σ.(world) g ∗
               trace_frag σ.(trace) ∗ oracle_frag σ.(oracle) ={⊤}=∗
@@ -190,7 +259,7 @@ Proof.
     iApply big_sepL_fmap.
     iApply (big_sepL_mono with "Hwp").
     iIntros (i (e&σ) Hlookup) "H".
-    iIntros (??) "Hres". iMod ("H" with "[$]") as "Hwp".
+    iIntros (???) "Hres". iMod ("H" $! _ _ with "[$]") as "Hwp".
     iDestruct "Hwp" as (Φ) "H".
     simpl.
     iModIntro. iExists Φ, (λ _, True%I), (λ _ _, True%I).
@@ -204,6 +273,7 @@ Proof.
       iApply wpc_value; eauto.
     }
   }
+  Unshelve. eauto.
 Qed.
 
 End failstop.
