src/program_proof/memkv/memkv_put_proof.v
@@ -268,9 +268,11 @@ Proof.
 
       (* Get Q by using fupd *)
       unfold PreShardPut.
-      iApply ncfupd_wp.
-      iMod (ncfupd_mask_subseteq _) as "Hclose"; last iMod "Hpre".
+      iApply fupd_wp.
+      iMod (fupd_mask_subseteq Eo) as "Hclose".
       { done. }
+      rewrite -global_groveG_inv_conv'.
+      iMod "Hpre".
       iDestruct "Hpre" as (v0) "(Hkvptsto2 & HfupdQ)".
       iMod (kvptsto_update args.(PR_Value) with "Hkvptsto Hkvptsto2") as "[Hkvptsto Hkvptsto2]".
       iMod ("HfupdQ" with "Hkvptsto") as "Q".
@@ -291,6 +293,8 @@ Proof.
 
       wp_pures.
 
+      iApply (fupd_wp).
+      rewrite -global_groveG_inv_conv'.
       iMod (server_completes_request with "His_srv HreqInv Hγpre [Q] Hproc") as "HH".
       { done. }
       { done. }
@@ -304,6 +308,9 @@ Proof.
         done.
       }
       iDestruct "HH" as "(#Hreceipt & Hrpc)".
+      iModIntro.
+      rewrite global_groveG_inv_conv'.
+
 
       iDestruct ("HshardMap_sl_close" with "HshardMap_sl") as "HshardMap_sl".
       wp_loadField.
