src/program_proof/memkv/print_assumptions.v
@@ -1,0 +1,3 @@
+From Perennial.program_proof.memkv Require Import closed.
+
+Print Assumptions shard_boot1.
